reduction_directedHamiltonianCircuit_to_hamiltonianCircuit/left_lemma_aux_file.dfy
@@ -1,0 +1,229 @@
+include "reduction_hamiltonian_definitions.dfy"
+include "reduction_hamiltonian_rFunction.dfy"
+include "permutation_property.dfy"
+include "reduction_hamiltonian_rCompletness.dfy"
+include "left_lemma_working_file.dfy"
+
+module LeftLemmaAux
+{
+    import opened Definitions
+    import opened ReductionFunction
+    import opened PermutationProperty
+    import opened ReductionCompletness
+    import opened LeftLemma
+
+    /**
+    We must ensure a standard circuit (oneWay and starting on in).
+        1. Verify that every circuit in the graph is either oneWay or otherWay (oneWayOrAnother_lemma).
+        2. For a circuit otherWay reverse it to make it oneWay (reverse_way_property_lemma).
+        3. For a circuit oneWay starting in other node cicle the sequence to start at an in_node (circuit_circular_property_lemma).
+     */
+
+    ghost function std_in_out_circuit(g: Graph): seq<nat>
+        requires validUndirectedGraph(g)
+        requires |g|>2 && |g|%3==0
+        requires in_out_graph(g)
+        requires undirectedHamiltonianCircuit(g)
+        ensures isUndirectedHamiltonianCircuit(g, std_in_out_circuit(g))
+        ensures standarized_in_out_circuit(g, std_in_out_circuit(g))
+    {
+        var c :| isUndirectedHamiltonianCircuit(g, c);
+        startAtIn(g, makeOneWay(g, c))
+    }
+
+    ghost function makeOneWay(g: Graph, c: seq<nat>): seq<nat>
+        requires validUndirectedGraph(g)
+        requires |g|>2 && |g|%3==0
+        requires in_out_graph(g)
+        requires isUndirectedHamiltonianCircuit(g, c)
+        ensures isUndirectedHamiltonianCircuit(g, makeOneWay(g, c))
+        ensures oneWay(g, makeOneWay(g, c))
+    {
+        oneWayOrAnother_lemma(g, c);
+        if oneWay(g, c) then c else circuit_reverse_property_lemma(g, c); reverse_way_property_lemma(g, c); rSeq(c)
+    }
+
+    ghost function startAtIn(g: Graph, c: seq<nat>): seq<nat>
+        requires validUndirectedGraph(g)
+        requires |g|>2 && |g|%3==0
+        requires in_out_graph(g)
+        requires isUndirectedHamiltonianCircuit(g, c)
+        requires oneWay(g, c)
+        ensures isUndirectedHamiltonianCircuit(g, startAtIn(g, c))
+        ensures oneWay(g, c)
+        ensures isInNode(g, startAtIn(g, c)[0])
+
+    //if there is a node k that doesn't satisfy in->og->out order then neither of the nodes satisfy that order
+    lemma aux_lemma(g: Graph, p: seq<nat>, k: nat)
+        requires validUndirectedGraph(g)
+        requires |g|>2 && |g|%3==0
+        requires in_out_graph(g)
+        // requires isUndirectedHamiltonianCircuit(g, c)
+        // requires !isOneWayPath(g, p)
+        requires 0<=k<|p|-1
+        requires
+            !(
+                (isInNode(g, p[k]) ==> isOgNode(g, p[k+1]))   //if this in next og
+                &&
+                (isOgNode(g, p[k]) ==> isOutNode(g, p[k+1]))   //if this og next out
+                &&
+                (isOutNode(g, p[k]) ==> isInNode(g, p[k+1]))   //if this out next in
+            )
+        ensures forall i :: 0<=i<|p|-1 ==>
+                !(
+                    (isInNode(g, p[i]) ==> isOgNode(g, p[i+1]))   //if this in next og
+                    &&
+                    (isOgNode(g, p[i]) ==> isOutNode(g, p[i+1]))   //if this og next out
+                    &&
+                    (isOutNode(g, p[i]) ==> isInNode(g, p[i+1]))   //if this out next in
+                )
+    {}
+
+    lemma oneWayOrAnother_lemma(g: Graph, c: seq<nat>)
+        requires validUndirectedGraph(g)
+        requires |g|>2 && |g|%3==0
+        requires in_out_graph(g)
+        requires isUndirectedHamiltonianCircuit(g, c)
+        ensures oneWay(g, c) || otherWay(g, c)
+    {
+
+        if !oneWay(g, c)
+            //must ensure otherWay(g, c)
+        {
+            // assert forall i :: 0<i<|c| ==> (g[c[i-1]][c[i]]) || (g[c[i]][c[i-1]]);
+            // assert
+            //     !(forall i :: 0<=i<|g|-1 ==>
+            //     (
+            //         (isInNode(g, c[i]) ==> isOgNode(g, c[i+1]))   //if this in next og
+            //         &&
+            //         (isOgNode(g, c[i]) ==> isOutNode(g, c[i+1]))   //if this og next out
+            //         &&
+            //         (isOutNode(g, c[i]) ==> isInNode(g, c[i+1]))   //if this out next in
+            //     ));
+            // var k :| 0<=k<|g|-1 && //use later at the forall /////
+            //     !(
+            //         (isInNode(g, c[k]) ==> isOgNode(g, c[k+1]))   //if this in next og
+            //         &&
+            //         (isOgNode(g, c[k]) ==> isOutNode(g, c[k+1]))   //if this og next out
+            //         &&
+            //         (isOutNode(g, c[k]) ==> isInNode(g, c[k+1]))   //if this out next in
+            //     );
+            
+            // forall i /*{:trigger i}*/ | 0<=i<|g|-1
+            //     ensures otherWay(g, c)
+            // {
+            //     assert (g[c[i]][c[i+1]] || g[c[i+1]][c[i]]);
+            //     if isInNode(g, c[i])
+            //     {
+            //         //in_out definition:
+            //         reveal in_out_graph(g);
+                    
+            //         assert (|g|/3)*2<=c[i]< |g|;
+            //         assert forall f :: 0<=f<|g|/3 ==> (forall c :: 0<=c<|g| ==> (c==f+(|g|/3)*2 ==> g[f][c]));
+            //         var n :| 0<=n<|g| && g[n][c[i]];
+
+            //         assert g[n][c[i]];
+            //         // assert g[c[i]-|g|/3][c[i]];
+            //         // assert g[c[i]-(|g|/3)*2][c[i]];
+            //         // assert isOgNode(g, c[i+1]) || isOutNode(g, c[i+1]);
+            //     }
+            }
+
+            assume otherWay(g, c);
+        }
+
+        // if !(oneWay(g, c) || otherWay(g, c))
+        // {
+        //     assert !oneWay(g, c) && !otherWay(g, c);
+        //     assert forall i :: 0<i<|c| ==> (g[c[i-1]][c[i]]) || (g[c[i]][c[i-1]]);
+        //     assert
+        //         !(forall i :: 0<=i<|g|-1 ==>
+        //         (
+        //             (isInNode(g, c[i]) ==> isOgNode(g, c[i+1]))   //if this in next og
+        //             &&
+        //             (isOgNode(g, c[i]) ==> isOutNode(g, c[i+1]))   //if this og next out
+        //             &&
+        //             (isOutNode(g, c[i]) ==> isInNode(g, c[i+1]))   //if this out next in
+        //         ))
+        //         &&
+        //         !(forall i :: 0<=i<|g|-1 ==>
+        //         (
+        //             (isOutNode(g, c[i]) ==> isOgNode(g, c[i+1]))   //if this out next og
+        //             &&
+        //             (isOgNode(g, c[i]) ==> isInNode(g, c[i+1]))   //if this og next in
+        //             &&
+        //             (isInNode(g, c[i]) ==> isOutNode(g, c[i+1]))   //if this in next out
+        //         ))
+        //         ;
+        //     assert exists i :: 0<=i<|g|-1 &&
+        //         !(
+        //             (isInNode(g, c[i]) ==> isOgNode(g, c[i+1]))   //if this in next og
+        //             &&
+        //             (isOgNode(g, c[i]) ==> isOutNode(g, c[i+1]))   //if this og next out
+        //             &&
+        //             (isOutNode(g, c[i]) ==> isInNode(g, c[i+1]))   //if this out next in
+        //         );
+        //     // assert exists i :: 0<=i<|g|-1 &&
+        //     //     !(
+        //     //         (isOutNode(g, c[i]) ==> isOgNode(g, c[i+1]))   //if this out next og
+        //     //         &&
+        //     //         (isOgNode(g, c[i]) ==> isInNode(g, c[i+1]))   //if this og next in
+        //     //         &&
+        //     //         (isInNode(g, c[i]) ==> isOutNode(g, c[i+1]))   //if this in next out
+        //     //     );
+            
+        //     var i :| 0<=i<|g|-1 &&
+        //         !(
+        //             (isInNode(g, c[i]) ==> isOgNode(g, c[i+1]))   //if this in next og
+        //             &&
+        //             (isOgNode(g, c[i]) ==> isOutNode(g, c[i+1]))   //if this og next out
+        //             &&
+        //             (isOutNode(g, c[i]) ==> isInNode(g, c[i+1]))   //if this out next in
+        //         );
+            
+        //     assert (g[c[i]][c[i+1]] || g[c[i+1]][c[i]]);
+        //     // (forall f :: (|g|/3)*2<=f<|g| ==> (forall c :: (|g|/3)*2<=c<|g| ==> !g[f][c]));    //no vertex from in to in
+
+
+        //     assume !isUndirectedHamiltonianCircuit(g, c);
+        // }
+    // }
+
+    ghost function rSeq(s: seq<nat>): seq<nat>
+    {
+        if |s| == 0 then
+            []
+        else
+            rSeq(s[1..]) + [s[0]]
+    }
+
+    lemma circuit_reverse_property_lemma(g: Graph, c: seq<nat>)
+        requires validUndirectedGraph(g)
+        requires |g|>2
+        requires isUndirectedHamiltonianCircuit(g, c)
+        ensures isUndirectedHamiltonianCircuit(g, c)
+    {}
+
+    ghost function cicle_sequence(s: seq<nat>, i: int): seq<nat>
+        requires 0<=i<|s|
+    {
+        s[i..|s|] + s[0..i]
+    }
+
+    lemma circuit_circular_property_lemma(g: Graph, c: seq<nat>)
+        requires validUndirectedGraph(g)
+        requires |g|>2
+        requires isUndirectedHamiltonianCircuit(g, c)
+        ensures forall i :: 0<=i<|c| ==> isUndirectedHamiltonianCircuit(g, cicle_sequence(c, i))
+    {}
+
+    lemma reverse_way_property_lemma(g: Graph, c: seq<nat>)
+        requires validUndirectedGraph(g)
+        requires |g|>2 && |g|%3==0
+        requires in_out_graph(g)
+        requires isUndirectedHamiltonianCircuit(g, c)
+        requires otherWay(g, c)
+        ensures oneWay(g, rSeq(c))
+    //TODO
+
+}
